reorganize file

iocy/iocy.fst
@@ -4,13 +4,133 @@ open FStar.Tactics
 open FStar.List.Tot.Base
 
 type trace (e:Type0) = list e
-  
+
 type run 'e (a:Type u#a) =
 | Cv : a -> trace 'e -> run 'e a
 
 noeq
 type runtree 'e (a:Type u#a) : Type u#a =
 | Node : run 'e a -> list (runtree 'e (Universe.raise_t unit)) -> runtree 'e a
+
+let rec univ_ch (t:runtree 'e (Universe.raise_t u#0 u#a unit)) : runtree 'e (Universe.raise_t u#0 u#b unit) =
+match t with
+| Node (Cv x tl) rts -> Node (Cv (Universe.raise_val (Universe.downgrade_val x)) tl) (univ_change rts)
+and univ_change (t:list u#a (runtree 'e (Universe.raise_t u#0 u#a unit))) : list u#b (runtree 'e (Universe.raise_t u#0 u#b unit)) =
+  (** map univ_ch t **)
+  match t with
+  | [] -> []
+  | h :: tl -> [univ_ch h]@(univ_change tl)
+
+type hist_post 'e 'a = runtree 'e 'a -> Type0
+type hist_pre 'e (a:Type u#a) = list (runtree 'e (Universe.raise_t u#0 u#a unit)) -> trace 'e -> Type0
+
+type hist0 'e 'a = hist_post 'e 'a -> hist_pre 'e 'a
+
+let hist_post_ord (p1 p2:hist_post 'e 'a) = forall r. p1 r ==> p2 r
+
+let hist_wp_monotonic (wp:hist0 'e 'a) =
+  forall p1 p2. (p1 `hist_post_ord` p2) ==> (forall ths h. wp p1 ths h ==> wp p2 ths h)
+
+type hist 'e 'a = wp:(hist0 'e 'a){hist_wp_monotonic wp}
+
+let hist_return (#e:Type0) (x:'a) : hist e 'a =
+  fun p _ _ -> p (Node (Cv x []) [])
+
+let hist_post_shift (p:hist_post 'e 'b) (rt:runtree 'e 'a) : hist_post 'e 'b =
+  fun (rt':runtree 'e 'b) -> 
+    match rt, rt' with
+    | Node (Cv x lt) trt, Node (Cv x' lt') trt' -> p (Node (Cv x' (lt@lt')) ((univ_change trt) @ trt'))
+
+let hist_post_bind
+  (#a:Type u#a) (#b:Type u#b)
+  (ths:list (runtree 'e (Universe.raise_t u#0 u#b unit)))
+  (h:trace 'e)
+  (kw : a -> hist 'e b)
+  (p:hist_post 'e b) :
+  Tot (hist_post 'e a) =
+  fun (rt:runtree 'e a) ->
+    match rt with | Node (Cv x lt) rts ->
+    kw x (hist_post_shift p rt) ((univ_change rts)@ths) (List.rev lt @ h)
+
+let hist_bind (#a:Type u#a) (#b:Type u#b) (w : hist 'e a) (kw : a -> hist 'e b) : hist 'e b =
+  let wp = fun p ths h -> w (hist_post_bind ths h kw p) (univ_change ths) h in
+  assume (hist_wp_monotonic wp);
+  wp
+
+noeq
+type free (a:Type u#a) (e:Type0) : Type u#(max 1 a)=
+| Require : (pre:pure_pre) -> cont:((squash pre) -> free u#a a e) -> free a e
+| Return : a -> free a e
+| Print : (arg:e) -> cont:(unit -> free u#a a e) -> free a e
+| Fork : th:(unit -> free (Universe.raise_t unit) e) -> cont:(unit -> free a e) -> free a e
+| Wait : nat -> cont:(option unit -> free a e) -> free a e
+
+let free_return (#a:Type) (#e:Type) (x:a) : free a e =
+  Return x
+
+let rec free_bind
+  (#a:Type u#a)
+  (#b:Type u#b)
+  (#e:Type)
+  (l : free a e)
+  (k : a -> free b e) :
+  free b e =
+  match l with
+  | Return x -> k x
+  | Print str fnc -> 
+      Print str (fun i -> free_bind (fnc i) k)
+  | Fork th fnc ->
+      Fork
+        (fun i -> free_bind #(Universe.raise_t u#0 u#a unit) #(Universe.raise_t u#0 u#b unit) #e (th i) (fun x -> free_return (Universe.raise_val u#0 u#b (Universe.downgrade_val x))))
+        (fun _ -> free_bind (fnc ()) k)
+  | Require pre fnc ->
+      Require pre (fun _ -> free_bind (fnc ()) k)
+  | Wait id fnc -> 
+      Wait id (fun i -> free_bind (fnc i) k)
+
+let hist_require #e (pre:pure_pre) : hist e (squash pre) = 
+  let wp' : hist0 e (squash pre) = fun p _ _ -> pre /\ p (Node (Cv () []) []) in
+  assert (forall post1 post2. (hist_post_ord post1 post2 ==> (forall h thrs. wp' post1 thrs h ==> wp' post2 thrs h)));
+  assert (hist_wp_monotonic wp');
+  wp'
+
+let hist_print (#e:Type) (ev:e) : hist e unit =
+  fun p _ _ -> p (Node (Cv () [ev]) [])
+
+let hist_fork (#e:Type u#0) (#a:Type u#a) (hist_th:hist e (Universe.raise_t u#0 u#a unit)) : hist e (Universe.raise_t u#0 u#a unit) =
+  let wp = fun p -> hist_th (fun r -> p (Node (Cv (Universe.raise_val ()) []) [r])) in
+  assume (hist_wp_monotonic wp);
+  wp
+
+val theta : (trace 'e -> runtree 'e (Universe.raise_t unit) -> Type0) -> free 'a 'e -> hist 'e 'a
+let rec theta sat m =
+  match m with
+  | Require pre k ->
+      hist_bind (hist_require pre) (fun r -> theta sat (k r))
+  | Return x -> hist_return x
+  | Print arg k ->
+      hist_bind (hist_print arg) (fun r -> theta sat (k r))
+  | Fork th k -> (
+    let wp = fun p thrs h -> 
+      theta sat (th ()) (fun rt -> 
+        theta sat (k ()) (fun rt' -> 
+          let (Node (Cv x lt) thrs) = rt' in
+          p (Node (Cv x []) [rt; (Node (Cv (Universe.raise_val ()) lt) thrs) ])
+        ) ((univ_ch rt)::thrs) h
+      ) thrs h in
+    assume (hist_wp_monotonic wp);
+    wp
+  )
+  | Wait id k -> let wp = (fun p thrds h ->
+    match nth thrds id with
+    | None -> theta sat (k None) p thrds h 
+    | Some rt ->
+    (forall lt. lt `sat` (univ_ch rt) ==>
+      theta sat (k (Some ())) (fun (Node (Cv x lt') rts) -> p (Node (Cv x (** append event with id**) lt') rts)) thrds (** - rt **) (List.rev lt @ h))) in
+    assume (hist_wp_monotonic wp);
+    wp
+
+
 
 let rec interleave (t1:trace 'e) (t2:trace 'e) : list (trace 'e) =
   match t1, t2 with
@@ -110,185 +230,53 @@ let _ =
       [5; 6; 0; 1; 2]; [5; 0; 6; 1; 2]; [5; 0; 1; 6; 2]; [5; 0; 1; 2; 6]; [0; 5; 6; 1; 2];
       [0; 5; 1; 6; 2]; [0; 5; 1; 2; 6]; [0; 1; 5; 6; 2]; [0; 1; 5; 2; 6]; [0; 1; 2; 5; 6]]) by (compute ())
 
+let theta' = theta (fun lt rt -> lt `List.memP` as_traces rt)
 
-let rec univ_ch (t:runtree 'e (Universe.raise_t u#0 u#a unit)) : runtree 'e (Universe.raise_t u#0 u#b unit) =
-match t with
-| Node (Cv x tl) rts -> Node (Cv (Universe.raise_val (Universe.downgrade_val x)) tl) (univ_change rts)
-and univ_change (t:list u#a (runtree 'e (Universe.raise_t u#0 u#a unit))) : list u#b (runtree 'e (Universe.raise_t u#0 u#b unit)) =
-  (** map univ_ch t **)
-  match t with
-  | [] -> []
-  | h :: tl -> [univ_ch h]@(univ_change tl)
-
-let rec prepend_rt (lt:list 'e) (rt:runtree 'e 'a) : Tot (runtree 'e 'a) (decreases rt) =
-  admit ();
-  match rt with
-  | Node (Cv x lt') rt -> Node (Cv x (lt@lt')) (map #(runtree 'e (Universe.raise_t unit)) (prepend_rt lt) rt)
-
-type hist_post 'e 'a = runtree 'e 'a -> Type0
-type hist_pre 'e (a:Type u#a) = list (runtree 'e (Universe.raise_t u#0 u#a unit)) -> trace 'e -> Type0
-
-type hist0 'e 'a = hist_post 'e 'a -> hist_pre 'e 'a
-
-let hist_post_ord (p1 p2:hist_post 'e 'a) = forall r. p1 r ==> p2 r
-
-let hist_wp_monotonic (wp:hist0 'e 'a) =
-  forall p1 p2. (p1 `hist_post_ord` p2) ==> (forall ths h. wp p1 ths h ==> wp p2 ths h)
-
-type hist 'e 'a = wp:(hist0 'e 'a){hist_wp_monotonic wp}
-
-let hist_return (#e:Type0) (x:'a) : hist e 'a =
-  fun p _ _ -> p (Node (Cv x []) [])
-
-let hist_post_shift (p:hist_post 'e 'b) (rt:runtree 'e 'a) : hist_post 'e 'b =
-  fun (rt':runtree 'e 'b) -> 
-    match rt, rt' with
-    | Node (Cv x lt) trt, Node (Cv x' lt') trt' -> p (Node (Cv x' (lt@lt')) ((univ_change trt) @ trt'))
-
-let hist_post_bind
-  (#a:Type u#a) (#b:Type u#b)
-  (ths:list (runtree 'e (Universe.raise_t u#0 u#b unit)))
-  (h:trace 'e)
-  (kw : a -> hist 'e b)
-  (p:hist_post 'e b) :
-  Tot (hist_post 'e a) =
-  fun (rt:runtree 'e a) ->
-    match rt with | Node (Cv x lt) rts ->
-    kw x (hist_post_shift p rt) ((univ_change rts)@ths) (List.rev lt @ h)
-
-let hist_bind0 (#a:Type u#a) (#b:Type u#b) (w : hist 'e a) (kw : a -> hist 'e b) : hist0 'e b =
-  fun p ths h -> w (hist_post_bind ths h kw p) (univ_change ths) h
-
-let hist_bind (#a:Type u#a) (#b:Type u#b) (w : hist 'e a) (kw : a -> hist 'e b) : hist 'e b =
-  let wp =   hist_bind0 w kw in
-  assume (hist_wp_monotonic wp);
-  wp
-
-val hist_ord : hist 'e 'a -> hist 'e 'a -> Type0
-let hist_ord wp1 wp2 = forall ths h p. wp1 p ths h ==> wp2 p ths h
-
-val hist_equiv : hist 'e 'a -> hist 'e 'a -> Type0
-let hist_equiv wp1 wp2 = forall h thrs p. wp1 p thrs h <==> wp2 p thrs h
-
-noeq
-type free (a:Type u#a) (e:Type0) : Type u#(max 1 a)=
-| Require : (pre:pure_pre) -> cont:((squash pre) -> free u#a a e) -> free a e
-| Return : a -> free a e
-| Print : (arg:e) -> cont:(unit -> free u#a a e) -> free a e
-| Fork : th:(unit -> free (Universe.raise_t unit) e) -> cont:(unit -> free a e) -> free a e
-| Wait : nat -> cont:(unit -> free a e) -> free a e
-
-let free_return (#a:Type) (#e:Type) (x:a) : free a e =
-  Return x
-
-let rec free_bind
-  (#a:Type u#a)
-  (#b:Type u#b)
-  (#e:Type)
-  (l : free a e)
-  (k : a -> free b e) :
-  free b e =
-  match l with
-  | Return x -> k x
-  | Print str fnc ->
-      Print str (fun i ->
-        free_bind (fnc i) k)
-  | Fork th fnc ->
-      Fork
-        (fun i -> free_bind #(Universe.raise_t u#0 u#a unit) #(Universe.raise_t u#0 u#b unit) #e (th i) (fun x -> free_return (Universe.raise_val u#0 u#b (Universe.downgrade_val x))))
-        (fun _ -> free_bind (fnc ()) k)
-  | Require pre fnc ->
-      Require pre (fun _ ->
-        free_bind (fnc ()) k)
-  | Wait id fnc ->
-      Wait id (fun i -> free_bind (fnc i) k)
-
-let hist_require #e (pre:pure_pre) : hist e (squash pre) = 
-  let wp' : hist0 e (squash pre) = fun p _ _ -> pre /\ p (Node (Cv () []) []) in
-  assert (forall post1 post2. (hist_post_ord post1 post2 ==> (forall h thrs. wp' post1 thrs h ==> wp' post2 thrs h)));
-  assert (hist_wp_monotonic wp');
-  wp'
-
-let hist_print (#e:Type) (ev:e) : hist e unit =
-  fun p _ _ -> p (Node (Cv () [ev]) [])
-
-let hist_fork0 (#e:Type u#0) (#a:Type u#a) (hist_th:hist e (Universe.raise_t u#0 u#a unit)) : hist0 e (Universe.raise_t u#0 u#a unit) =
-  fun p -> hist_th (fun r -> p (Node (Cv (Universe.raise_val ()) []) [r]))
-
-let hist_fork (#e:Type u#0) (#a:Type u#a) (hist_th:hist e (Universe.raise_t u#0 u#a unit)) : hist e (Universe.raise_t u#0 u#a unit) =
-  let wp = hist_fork0 #e #a hist_th in
-  assume (hist_wp_monotonic wp);
-  wp
-
-val theta : free 'a 'e -> hist 'e 'a
-let rec theta m =
-  match m with
-  | Require pre k ->
-      hist_bind (hist_require pre) (fun r -> theta (k r))
-  | Return x -> hist_return x
-  | Print arg k ->
-      hist_bind (hist_print arg) (fun r -> theta (k r))
-  | Fork th k -> (
-    let wp = fun p thrs h -> 
-      theta (th ()) (fun rt -> 
-        theta (k ()) (fun rt' -> 
-          let (Node (Cv x lt) thrs) = rt' in
-          p (Node (Cv x []) [rt; (Node (Cv (Universe.raise_val ()) lt) thrs) ])
-        ) ((univ_ch rt)::thrs) h
-      ) thrs h in
-    assume (hist_wp_monotonic wp);
-    wp
-  )
-  | Wait id k -> let wp = (fun p thrds h ->
-    match nth thrds id with
-    | None -> True 
-    | Some rt ->
-    (forall lt. lt `memP` as_traces rt ==>
-      theta (k ()) (fun (Node (Cv x lt') rts) -> p (Node (Cv x lt') rts)) thrds (** - rt **) (List.rev lt @ h))) in
-    assume (hist_wp_monotonic wp);
-    wp
-
-
+(** *** Tests **)
 let result (r:runtree 'e 'a) : 'a =
   match r with
   | Node (Cv x _) _ -> x
   
 let prog0 =  Print 0 (fun () -> Print 1 (fun () -> Print 2 (fun () -> Return 5)))
 
-let _ = assert (theta prog0 (fun r -> result r == 5 /\ as_traces r === [[0; 1; 2]]) [] [])  by (compute ())
+let _ = assert (theta' prog0 (fun r -> result r == 5 /\ as_traces r === [[0; 1; 2]]) [] [])  by (compute ())
 
 let prog1 = Fork (fun () -> Print 0 (fun () -> Return (Universe.raise_val ()))) 
                  (fun () -> Print 1 (fun () -> Fork (fun () -> Print 2 (fun () -> Return (Universe.raise_val ())))
                                                   (fun () -> Return ())))
 
 
-let _ = assert (theta prog1 (fun r -> as_traces r === [[1; 0; 2]; [1; 2; 0]; [0; 1; 2]]) [] []) by (compute ())
+let _ = assert (theta' prog1 (fun r -> as_traces r === [[1; 0; 2]; [1; 2; 0]; [0; 1; 2]]) [] []) by (compute ())
 
 let prog2 =  Print 0 
                  (fun () -> Print 1 (fun () -> Fork (fun () -> Print 2 (fun () -> Return (Universe.raise_val ())))
                                                 (fun () -> Return 5)))
 
-let _ = assert (theta prog2 (fun r -> result r == 5 /\ as_traces r === [[0; 1; 2]]) [] [])  by (compute ())
+let _ = assert (theta' prog2 (fun r -> result r == 5 /\ as_traces r === [[0; 1; 2]]) [] [])  by (compute ())
 
 
 let prog3 = Fork (fun () -> Print 0 (fun () -> Fork (fun () -> Print 2 (fun () -> Return (Universe.raise_val ())))
                                                  (fun () -> Return (Universe.raise_val ()))))
                  (fun () -> Print 1 (fun () -> Return ()))
 
-let _ = assert (theta prog3 (fun r -> result r == () /\ as_traces r === [[0; 2; 1];[0;1;2];[1;0;2]]) [] []) by (compute ())
+let _ = assert (theta' prog3 (fun r -> result r == () /\ as_traces r === [[0; 2; 1];[0;1;2];[1;0;2]]) [] []) by (compute ())
 
+(** TODO: extra test, check if the history after Wait can be 0,5 and 5,0, not just 5,0 **)
 let prog4 = Fork (fun () -> Print 0 (fun () -> Return (Universe.raise_val ()))) 
-                 (fun () -> Print 5 (fun () -> Wait 0 (fun () -> Print 6 (fun () -> Return ()))))
+                 (fun () -> Print 5 (fun () -> Wait 0 (fun _ -> Print 6 (fun () -> Return ()))))
 
-let _ = assert (theta prog4 (fun r -> result r == () /\ as_traces r == [[0; 5; 6];[5;0;6]]) [] [])  by (  compute ();
+let _ = assert (theta' prog4 (fun r -> result r == () /\ as_traces r == [[0; 5; 6];[5;0;6]]) [] [])  by (  compute ();
   dump "h";
   tadmit ())
 
 let prog5 = Fork (fun () -> Print 0 (fun () -> Fork (fun () -> Print 1 (fun () -> Return (Universe.raise_val ())))
                                                  (fun () -> Print 2 (fun () -> Return (Universe.raise_val ())))))
-                 (fun () -> Print 5 (fun () -> Wait 0 (fun () -> Print 6 (fun () -> Return ()))))
+                 (fun () -> Print 5 (fun () -> Wait 0 (fun _ -> Print 6 (fun () -> Return ()))))
 
 
-let _ = assert (theta prog5 (fun r -> result r == () /\ as_traces r == [[0;1;2;5;6];[0;2;1;5;6];[0;2;5;1;6];[0;5;2;1;6];[0;5;2;1;6]]) [] [])  by (
+let _ = assert (theta' prog5 (fun r -> result r == () /\ as_traces r == [[0;1;2;5;6];[0;2;1;5;6];[0;2;5;1;6];[0;5;2;1;6];[0;5;2;1;6]]) [] [])  by (
   compute ();
   dump "h")
+
+
+(** TODO: test Fork followed by Fork **)
